holsrcs/sanityScript.sml
@@ -1,0 +1,134 @@
+(* Sanity theorems for the C++ semantics *)
+
+(* Michael Norrish *)
+
+(* pro-forma *)
+open HolKernel boolLib Parse bossLib BasicProvers
+open boolSimps
+
+(* Standard HOL ancestory theories *)
+open arithmeticTheory pred_setTheory integerTheory
+local open wordsTheory integer_wordTheory finite_mapTheory in end
+
+(* C++ ancestor theories  *)
+open dynamicsTheory
+local open side_effectsTheory statesTheory operatorsTheory in end
+
+val _ = new_theory "sanity";
+
+(* ----------------------------------------------------------------------
+    function info remains invariant
+
+    The meaning relation doesn't update the function map, only the
+    emeaning relation does.
+
+   ---------------------------------------------------------------------- *)
+
+open side_effectsTheory
+val val2mem_fnmap = store_thm(
+  "val2mem_fnmap",
+  ``(val2mem s a v).fnmap = s.fnmap``,
+  SRW_TAC [][statesTheory.val2mem_def]);
+val _ = export_rewrites ["val2mem_fnmap"]
+val apply_se_preserves_fnmaps = prove(
+  ``apply_se (se0,s0) (se,s) ==> (s0.fnmap = s.fnmap)``,
+    SRW_TAC [][apply_se_def, apply_lse_def] THEN
+    Cases_on `ise` THEN
+    FULL_SIMP_TAC (srw_ss()) [se_on_state_def])
+
+val rec_i_vars_preserves_fnmaps = prove(
+  ``!s0 vars s. rec_i_vars s0 vars s ==> (s0.fnmap = s.fnmap)``,
+  Induct_on `vars` THEN
+  ASM_SIMP_TAC (srw_ss()) [pairTheory.FORALL_PROD, rec_i_vars_def] THEN
+  REPEAT STRIP_TAC THEN RES_TAC THEN FULL_SIMP_TAC (srw_ss()) [])
+
+val rec_i_vals_preserves_fnmaps = prove(
+  ``!s0 prms vals s. rec_i_vals s0 prms vals s ==> (s0.fnmap = s.fnmap)``,
+  Induct_on `prms` THEN
+  ASM_SIMP_TAC (srw_ss()) [pairTheory.FORALL_PROD, rec_i_vals_def] THEN
+  REPEAT STRIP_TAC THEN RES_TAC THEN FULL_SIMP_TAC (srw_ss()) [])
+
+val pass_parameters_preserves_fnmaps = prove(
+  ``pass_parameters s0 fnid params s ==> (s0.fnmap = s.fnmap)``,
+  SRW_TAC [][pass_parameters_def, install_vars_def, install_values_def] THEN
+  MAP_EVERY IMP_RES_TAC [rec_i_vals_preserves_fnmaps,
+                         rec_i_vars_preserves_fnmaps] THEN
+  FULL_SIMP_TAC (srw_ss()) [])
+
+val vdeclare_preserves_fnmaps = prove(
+  ``vdeclare s0 ty name s ==> (s0.fnmap = s.fnmap)``,
+  SRW_TAC [][vdeclare_def] THEN SRW_TAC [][]);
+
+
+(* final result *)
+val fninfo_invariant = store_thm(
+  "fninfo_invariant",
+  ``!ee0 s0 see. meaning ee0 s0 see ==> (s0.fnmap = (FST see).fnmap)``,
+  HO_MATCH_MP_TAC meaning_ind THEN SRW_TAC [][] THEN
+  METIS_TAC [lval2rval_states_equal, apply_se_preserves_fnmaps,
+             pass_parameters_preserves_fnmaps, vdeclare_preserves_fnmaps]);
+
+(* ----------------------------------------------------------------------
+    class_lvalue_safe
+       If a class lvalue occurs, its type (Class cname) will have the same
+       cname as the last element of the accompanying path
+   ---------------------------------------------------------------------- *)
+
+val clval_safe_def = Define`
+  (clval_safe (LVal a (Class c) p) = ~(p = []) /\ (c = LAST p)) /\
+  (clval_safe e = T)
+`
+val _ = export_rewrites ["clval_safe_def"]
+
+val clvalue_safe_def = Define`
+  clvalue_safe e = rec_expr_P e clval_safe
+`;
+val _ = export_rewrites ["clvalue_safe_def"]
+
+(* this proof can't work until I come up with a way of describing memory
+   as being "safe" with respect to a program, meaning that any pointers
+   read out of memory and pointing to a class satisfy the safety property -
+   I suspect this may need to be axiomatised into the ptr_decode function,
+   such that if ptr_decode returns SOME (addr,p) then it's OK.  If it's NONE
+   then that means the pointer is bad, and the result is undefined behaviour *)
+
+(*
+val clvalue_safe_invariant = store_thm(
+  "clvalue_safe_invariant",
+  ``!e s sse. meaning e s sse ==>
+              erec_exte clvalue_safe e ==>
+              erec_exte clvalue_safe (SND sse)``,
+  HO_MATCH_MP_TAC meaning_ind THEN
+  SRW_TAC [][statementsTheory.erec_stmt_def,
+             expressionsTheory.rec_expr_P_def]  THEN
+  SRW_TAC [][expressionsTheory.rec_expr_P_def] THENL [
+    Cases_on `s.typemap ' vname` THEN
+    SRW_TAC [][statesTheory.default_path_def],
+
+    FULL_SIMP_TAC (srw_ss()) [valid_econtext_def] THEN
+    SRW_TAC [][] THEN
+    FULL_SIMP_TAC (srw_ss()) [expressionsTheory.rec_expr_P_def],
+
+    FULL_SIMP_TAC (srw_ss()) [valid_econtext_def] THEN
+    SRW_TAC [][] THEN
+    FULL_SIMP_TAC (srw_ss()) [expressionsTheory.rec_expr_P_def],
+
+    FULL_SIMP_TAC (srw_ss()) [valid_lvcontext_def] THEN
+    SRW_TAC [][] THEN
+    IMP_RES_TAC lval2rval_results THEN
+    FULL_SIMP_TAC (srw_ss()) [expressionsTheory.rec_expr_P_def],
+
+    SRW_TAC [][expressionsTheory.rec_expr_P_def],
+    SRW_TAC [][expressionsTheory.rec_expr_P_def],
+    SRW_TAC [][expressionsTheory.rec_expr_P_def],
+
+
+    FULL_SIMP_TAC (srw_ss()) [expressionsTheory.rec_expr_P_def],
+
+*)
+
+
+
+val _ = export_theory();
+
+
